tests/lean/run/premise_selection_mepo.lean
@@ -14,11 +14,22 @@ example (x y z : List Int) : x ++ y ++ z = x ++ (y ++ z) := by
 -- `useRarity` is too slow in practice: it requires analyzing all the types in the environment.
 -- It would need to be cached.
 
--- set_premise_selector Lean.PremiseSelection.mepoSelector (useRarity := true)
+open Lean
+run_meta do
+  let env ← getEnv
+  let i := Lean.PremiseSelection.MePo.symbolFrequency env ``Name
+  logInfo m!"{i}"
 
--- example (a b : Int) : a + b = b + a := by
---   suggest_premises
---   sorry
+run_meta do
+  let env ← getEnv
+  let n := Lean.PremiseSelection.MePo.symbolFrequencyExt.getState env |>.map fun as => as.size
+  logInfo m!"{n}"
+
+set_premise_selector Lean.PremiseSelection.mepoSelector (useRarity := true)
+
+example (a b : Int) : a + b = b + a := by
+  suggest_premises
+  sorry
 
 -- #time
 -- example (x y z : List Int) : x ++ y ++ z = x ++ (y ++ z) := by
